ironfleet/src/Dafny/Distributed/Concur/RemoveUpdates.i.dfy
@@ -1,0 +1,125 @@
+include "Reduction.i.dfy"
+include "RefinementConvolution.i.dfy"
+include "SystemRefinement.i.dfy"
+
+module RemoveUpdatesModule {
+
+    import opened ReductionModule
+    import opened RefinementConvolutionModule
+    import opened SystemRefinementModule
+
+    function {:opaque} MapSeqToSeq<T,U>(s:seq<T>, refine_func:T->U) : seq<U>
+        reads refine_func.reads;
+        requires forall i :: refine_func.reads(i) == {};
+        requires forall i :: 0 <= i < |s| ==> refine_func.requires(s[i]);
+        ensures |MapSeqToSeq(s, refine_func)| == |s|;
+        ensures forall i :: 0 <= i < |s| ==> refine_func(s[i]) == MapSeqToSeq(s,refine_func)[i];
+    {
+        if |s| == 0 then []
+        else [refine_func(s[0])] + MapSeqToSeq(s[1..], refine_func)
+    }
+
+    function RemoveActorStateFromSystemState(ds:SystemState) : SystemState
+    {
+        ds.(states := map[])
+    }
+
+    lemma lemma_SystemCorrespondenceBetweenSystemStateAndItselfWithoutActorStates(
+        ds:SystemState,
+        ds':SystemState
+        )
+        requires ds' == RemoveActorStateFromSystemState(ds);
+        ensures  SystemCorrespondence(ds, ds');
+        decreases |ds.states|;
+    {
+        if ds.states == map [] {
+            return;
+        }
+
+        var actor :| actor in ds.states;
+        var ds_mid := ds.(states := mapremove(ds.states, actor));
+        assert |ds_mid.states| == |ds.states| - 1;
+        var relation := GetSystemSystemRefinementRelation();
+        lemma_SystemCorrespondenceBetweenSystemStateAndItselfWithoutActorStates(ds_mid, ds');
+        assert RefinementPair(ds_mid, ds') in relation;
+
+        forall ss | SpecCorrespondence(ds_mid, ss)
+            ensures SpecCorrespondence(ds, ss);
+        {
+            var entry := Entry(actor, UpdateLocalState());
+            assert SystemNextEntry(ds, ds_mid, entry);
+            lemma_LeftMoverBackwardPreservation(entry, ds, ds_mid, ss);
+        }
+        assert SystemCorrespondence(ds, ds_mid);
+
+        assert RefinementPair(ds, ds_mid) in relation;
+        lemma_SystemRefinementRelationConvolvesWithItself();
+        assert RefinementPair(ds, ds') in relation;
+    }
+
+    lemma lemma_SystemNextEntryPreservedWhenRemovingActorState(
+        ds0:SystemState,
+        ds1:SystemState,
+        ds0':SystemState,
+        ds1':SystemState,
+        entry:Entry
+        )
+        requires SystemNextEntry(ds0, ds1, entry);
+        requires ds0' == RemoveActorStateFromSystemState(ds0);
+        requires ds1' == RemoveActorStateFromSystemState(ds1);
+        requires !entry.action.HostNext?;
+        ensures  SystemNextEntry(ds0', ds1', entry);
+    {
+    }
+
+    lemma lemma_GetTrivialRefinementMap(n:int) returns (lh_map:RefinementMap)
+        requires n >= 0;
+        ensures  IsValidRefinementMap(n, n, lh_map);
+        ensures  forall i {:trigger lh_map[i]} :: 0 <= i < n ==> lh_map[i] == RefinementRange(i, i);
+    {
+        if n == 0 {
+            lh_map := [];
+            return;
+        }
+
+        var lh_map' := lemma_GetTrivialRefinementMap(n-1);
+        lh_map := lh_map' + [RefinementRange(n-1, n-1)];
+    }
+
+    lemma lemma_RefineToBehaviorWithoutStates(
+        trace:Trace,
+        db:seq<SystemState>
+        ) returns (
+        trace':Trace,
+        db':seq<SystemState>
+        )
+        requires IsValidSystemTraceAndBehavior(trace, db);
+        requires forall entry :: entry in trace ==> IsRealAction(entry.action);
+        ensures  IsValidSystemTraceAndBehavior(trace', db');
+        ensures  SystemBehaviorRefinesSystemBehavior(db, db');
+        ensures  forall entry :: entry in trace' ==> IsRealAction(entry.action);
+        ensures  forall ds :: ds in db' ==> ds.states == map [];
+    {
+        trace' := trace;
+        db' := MapSeqToSeq(db, RemoveActorStateFromSystemState);
+        var lh_map := lemma_GetTrivialRefinementMap(|db|);
+        var relation := GetSystemSystemRefinementRelation();
+
+        forall i, j {:trigger RefinementPair(db[i], db'[j]) in relation} |
+            0 <= i < |db| && lh_map[i].first <= j <= lh_map[i].last && 0 <= j < |db'|
+            ensures RefinementPair(db[i], db'[j]) in relation;
+        {
+            assert j == i;
+            assert db'[j] == RemoveActorStateFromSystemState(db[i]);
+            lemma_SystemCorrespondenceBetweenSystemStateAndItselfWithoutActorStates(db[i], db'[j]);
+        }
+        assert BehaviorRefinesBehaviorUsingRefinementMap(db, db', relation, lh_map);
+
+        forall i {:trigger SystemNextEntry(db'[i], db'[i+1], trace'[i])} | 0 <= i < |db'|-1
+            ensures SystemNextEntry(db'[i], db'[i+1], trace'[i]);
+        {
+            lemma_SystemNextEntryPreservedWhenRemovingActorState(db[i], db[i+1], db'[i], db'[i+1], trace[i]);
+        }
+    }
+
+}
